execution/tests/TestUtils.v
@@ -577,7 +577,7 @@ Definition indepForAll4 {A B C D prop : Type}
                             pf.
 
 (* Little helper to avoid having to write out matches with "false ==> true" in None case all the time *)
-Definition isSomeCheck {A : Type} (a : option A) (f : A -> Checker) : Checker := 
+Definition isSomeCheck {A B : Type} `{Checkable B} (a : option A) (f : A -> B) : Checker := 
 match a with 
   | Some v => checker (f v)
   | None => false ==> true
